book/FPLean/Examples/OtherLanguages.lean
@@ -1,9 +1,10 @@
 import SubVerso.Examples
 import Lean.Data.NameMap
+import Std.Data.HashMap
 import VersoManual
 
 open Lean (NameMap MessageSeverity)
-
+open Std
 
 namespace FPLean
 
@@ -70,3 +71,76 @@ def inlineTypescript : RoleExpander
     let `(inline|code($code)) := code
       | throwErrorAt code "Exected code"
     return #[← ``(Inline.code $(quote code.getString))]
+
+section
+
+variable [Monad m] [MonadError m]
+
+structure IncludePythonConfig where
+  file : String
+  anchor? : Option Ident
+
+instance : FromArgs IncludePythonConfig m where
+  fromArgs :=   IncludePythonConfig.mk <$> .positional' `file <*> .named' `anchor true
+
+end
+
+/--
+If a line could be an anchor indicator, returns the anchor's name along with `true` for a start
+and `false` for an end.
+
+An anchor consists of a line that contains `ANCHOR:` or `ANCHOR_END:` followed by the name
+of the anchor.
+-/
+def anchor? (line : String) : Except String (String × Bool) := do
+  let mut line := line.trim
+  line := line.dropWhile (· ≠ 'A')
+  if line.startsWith "ANCHOR:" then
+    line := line.stripPrefix "ANCHOR:"
+    line := line.trimLeft
+    if line.isEmpty then throw "Expected name after `ANCHOR: `" else return (line, true)
+  else if line.startsWith "ANCHOR_END:" then
+    line := line.stripPrefix "ANCHOR_END:"
+    line := line.trimLeft
+    if line.isEmpty then throw "Expected name after `ANCHOR_END: `" else return (line, false)
+  else throw s!"Expected `ANCHOR:` or `ANCHOR_END:`, got {line}"
+
+private def stringAnchors (s : String) : Except String (String × HashMap String String) := do
+  let mut out := ""
+  let mut anchors : HashMap String String := {}
+  let mut openAnchors : HashMap String String := {}
+  let lines := s.split (· == '\n')
+  for line in lines do
+    if let some (a, isOpener) := anchor? line |>.toOption then
+      if isOpener then
+        if openAnchors.contains a then throw s!"Already open: {a}"
+        else openAnchors := openAnchors.insert a ""
+      else
+        if let some txt := openAnchors[a]? then
+          anchors := anchors.insert a txt
+          openAnchors := openAnchors.erase a
+        else throw s!"Not open: {a}"
+    else
+      out := out ++ line ++ "\n"
+      for (k, v) in openAnchors do
+        openAnchors := openAnchors.insert k (v ++ line ++ "\n")
+  for a in openAnchors.keys do
+    throw s!"Anchor {a} never closed"
+  return (out, anchors)
+
+@[code_block_expander includePython]
+def includePython : CodeBlockExpander
+  | args, code => do
+    let {file, anchor?} ← parseThe IncludePythonConfig args
+    let s ← IO.FS.readFile file
+    let txt ←
+      if let some a := anchor? then
+        let .ok (_, as) := stringAnchors s
+          | throwErrorAt a m!"Couldn't parse anchors"
+        let some txt := as[a.getId.eraseMacroScopes.toString]?
+          | throwErrorAt a m!"Not found in {as.keys}"
+        pure txt
+      else
+        pure s
+    _ ← ExpectString.expectString "file" code txt
+    return #[← ``(Block.code $(quote code.getString))]
