book/FPLean/Monads/Class.lean
@@ -1,0 +1,294 @@
+import VersoManual
+import FPLean.Examples
+
+open Verso.Genre Manual ExternalLean
+
+open FPLean
+
+set_option verso.exampleProject "../examples"
+set_option verso.exampleModule "Examples.Monads.Class"
+set_option verso.externalExamples.suppressedNamespaces "Class Errs IdentMonad MyListStuff One Two Three Four FourPointFive Temp TTT MonadLaws Exercises Busted"
+
+#doc (Manual) "The Monad Type Class" =>
+
+:::paragraph
+Rather than having to import an operator like `ok` or `andThen` for each type that is a monad, the Lean standard library contains a type class that allow them to be overloaded, so that the same operators can be used for _any_ monad.
+Monads have two operations, which are the equivalent of `ok` and `andThen`:
+
+```anchor FakeMonad
+class Monad (m : Type → Type) where
+  pure : α → m α
+  bind : m α → (α → m β) → m β
+```
+This definition is slightly simplified.
+The actual definition in the Lean library is somewhat more involved, and will be presented later.
+:::
+
+:::paragraph
+The {anchorName MonadOptionExcept}`Monad` instances for {anchorName MonadOptionExcept}`Option` and {anchorTerm MonadOptionExcept}`Except ε` can be created by adapting the definitions of their respective `andThen` operations:
+
+```anchor MonadOptionExcept
+instance : Monad Option where
+  pure x := some x
+  bind opt next :=
+    match opt with
+    | none => none
+    | some x => next x
+
+instance : Monad (Except ε) where
+  pure x := Except.ok x
+  bind attempt next :=
+    match attempt with
+    | Except.error e => Except.error e
+    | Except.ok x => next x
+```
+:::
+
+:::paragraph
+As an example, `firstThirdFifthSeventh` was defined separately for {anchorTerm Names}`Option α` and {anchorTerm Names}`Except String α` return types.
+Now, it can be defined polymorphically for _any_ monad.
+It does, however, require a lookup function as an argument, because different monads might fail to find a result in different ways.
+The infix version of {anchorName FakeMonad}`bind` is `>>=`, which plays the same role as `~~>` in the examples.
+
+```anchor firstThirdFifthSeventhMonad
+def firstThirdFifthSeventh [Monad m] (lookup : List α → Nat → m α) (xs : List α) : m (α × α × α × α) :=
+  lookup xs 0 >>= fun first =>
+  lookup xs 2 >>= fun third =>
+  lookup xs 4 >>= fun fifth =>
+  lookup xs 6 >>= fun seventh =>
+  pure (first, third, fifth, seventh)
+```
+:::
+
+:::paragraph
+Given example lists of slow mammals and fast birds, this implementation of {anchorName firstThirdFifthSeventhMonad}`firstThirdFifthSeventh` can be used with {moduleName}`Option`:
+
+```anchor animals
+def slowMammals : List String :=
+  ["Three-toed sloth", "Slow loris"]
+
+def fastBirds : List String := [
+  "Peregrine falcon",
+  "Saker falcon",
+  "Golden eagle",
+  "Gray-headed albatross",
+  "Spur-winged goose",
+  "Swift",
+  "Anna's hummingbird"
+]
+```
+```anchor noneSlow
+#eval firstThirdFifthSeventh (fun xs i => xs[i]?) slowMammals
+```
+```anchorInfo noneSlow
+none
+```
+```anchor someFast
+#eval firstThirdFifthSeventh (fun xs i => xs[i]?) fastBirds
+```
+```anchorInfo someFast
+some ("Peregrine falcon", "Golden eagle", "Spur-winged goose", "Anna's hummingbird")
+```
+:::
+
+:::paragraph
+After renaming {anchorName getOrExcept}`Except`'s lookup function `get` to something more specific, the very same implementation of {anchorName firstThirdFifthSeventhMonad}`firstThirdFifthSeventh` can be used with {anchorName getOrExcept}`Except` as well:
+
+```anchor getOrExcept
+def getOrExcept (xs : List α) (i : Nat) : Except String α :=
+  match xs[i]? with
+  | none => Except.error s!"Index {i} not found (maximum is {xs.length - 1})"
+  | some x => Except.ok x
+```
+```anchor errorSlow
+#eval firstThirdFifthSeventh getOrExcept slowMammals
+```
+```anchorInfo errorSlow
+Except.error "Index 2 not found (maximum is 1)"
+```
+```anchor okFast
+#eval firstThirdFifthSeventh getOrExcept fastBirds
+```
+```anchorInfo okFast
+Except.ok ("Peregrine falcon", "Golden eagle", "Spur-winged goose", "Anna's hummingbird")
+```
+The fact that {anchorName firstThirdFifthSeventhMonad}`m` must have a {anchorName firstThirdFifthSeventhMonad}`Monad` instance means that the `>>=` and {anchorName firstThirdFifthSeventhMonad}`pure` operations are available.
+:::
+
+# General Monad Operations
+
+:::paragraph
+Because many different types are monads, functions that are polymorphic over _any_ monad are very powerful.
+For example, the function {anchorName mapM}`mapM` is a version of {anchorName Names (show:=map)}`Functor.map` that uses a {anchorName mapM}`Monad` to sequence and combine the results of applying a function:
+
+```anchor mapM
+def mapM [Monad m] (f : α → m β) : List α → m (List β)
+  | [] => pure []
+  | x :: xs =>
+    f x >>= fun hd =>
+    mapM f xs >>= fun tl =>
+    pure (hd :: tl)
+```
+The return type of the function argument {anchorName mapM}`f` determines which {anchorName mapM}`Monad` instance will be used.
+In other words, {anchorName mapM}`mapM` can be used for functions that produce logs, for functions that can fail, or for functions that use mutable state.
+Because {anchorName mapM}`f`'s type determines the available effects, they can be tightly controlled by API designers.
+:::
+
+:::paragraph
+As described in [this chapter's introduction](../monads.md#numbering-tree-nodes), {anchorTerm StateEx}`State σ α` represents programs that make use of a mutable variable of type {anchorName StateEx}`σ` and return a value of type {anchorName StateEx}`α`.
+These programs are actually functions from a starting state to a pair of a value and a final state.
+The {anchorName StateMonad}`Monad` class requires that its parameter expect a single type argument—that is, it should be a {anchorTerm StateEx}`Type → Type`.
+This means that the instance for {anchorName StateMonad}`State` should mention the state type {anchorName StateMonad}`σ`, which becomes a parameter to the instance:
+
+```anchor StateMonad
+instance : Monad (State σ) where
+  pure x := fun s => (s, x)
+  bind first next :=
+    fun s =>
+      let (s', x) := first s
+      next x s'
+```
+This means that the type of the state cannot change between calls to {anchorName StateEx}`get` and {anchorName StateEx}`set` that are sequenced using {anchorName StateMonad}`bind`, which is a reasonable rule for stateful computations.
+The operator {anchorName increment}`increment` increases a saved state by a given amount, returning the old value:
+
+```anchor increment
+def increment (howMuch : Int) : State Int Int :=
+  get >>= fun i =>
+  set (i + howMuch) >>= fun () =>
+  pure i
+```
+:::
+
+:::paragraph
+Using {anchorName mapMincrementOut}`mapM` with {anchorName mapMincrementOut}`increment` results in a program that computes the sum of the entries in a list.
+More specifically, the mutable variable contains the sum so far, while the resulting list contains a running sum.
+In other words, {anchorTerm mapMincrement}`mapM increment` has type {anchorTerm mapMincrement}`List Int → State Int (List Int)`, and expanding the definition of `State` yields {anchorTerm mapMincrement2}`List Int → Int → (Int × List Int)`.
+It takes an initial sum as an argument, which should be {anchorTerm mapMincrementOut}`0`:
+```anchor mapMincrementOut
+#eval mapM increment [1, 2, 3, 4, 5] 0
+```
+```anchorInfo mapMincrementOut
+(15, [0, 1, 3, 6, 10])
+```
+:::
+
+:::paragraph
+A [logging effect](../monads.md#logging) can be represented using `WithLog`.
+Just like {anchorName StateEx}`State`, its {anchorName MonadWriter}`Monad` instance is polymorphic with respect to the type of the logged data:
+
+```anchor MonadWriter
+instance : Monad (WithLog logged) where
+  pure x := {log := [], val := x}
+  bind result next :=
+    let {log := thisOut, val := thisRes} := result
+    let {log := nextOut, val := nextRes} := next thisRes
+    {log := thisOut ++ nextOut, val := nextRes}
+```
+:::
+
+:::paragraph
+{anchorName saveIfEven}`saveIfEven` is a function that logs even numbers but returns its argument unchanged:
+
+```anchor saveIfEven
+def saveIfEven (i : Int) : WithLog Int Int :=
+  (if isEven i then
+    save i
+   else pure ()) >>= fun () =>
+  pure i
+```
+Using this function with {anchorName mapMsaveIfEven}`mapM` results in a log containing even numbers paired with an unchanged input list:
+```anchor mapMsaveIfEven
+#eval mapM saveIfEven [1, 2, 3, 4, 5]
+```
+```anchorInfo mapMsaveIfEven
+{ log := [2, 4], val := [1, 2, 3, 4, 5] }
+```
+:::
+
+
+# The Identity Monad
+
+Monads encode programs with effects, such as failure, exceptions, or logging, into explicit representations as data and functions.
+Sometimes, however, an API will be written to use a monad for flexibility, but the API's client may not require any encoded effects.
+The {tech}_identity monad_ is a monad that has no effects.
+It allows pure code to be used with monadic APIs:
+
+```anchor IdMonad
+def Id (t : Type) : Type := t
+
+instance : Monad Id where
+  pure x := x
+  bind x f := f x
+```
+The type of {anchorName IdMonad}`pure` should be {anchorTerm IdMore}`α → Id α`, but {anchorTerm IdMore}`Id α` reduces to just {anchorTerm IdMore}`α`.
+Similarly, the type of {anchorName IdMonad}`bind` should be {anchorTerm IdMore}`α → (α → Id β) → Id β`.
+Because this reduces to {anchorTerm IdMore}`α → (α → β) → β`, the second argument can be applied to the first to find the result.
+
+:::paragraph
+With the identity monad, {anchorName mapMId}`mapM` becomes equivalent to {anchorName Names (show:=map)}`Functor.map`
+To call it this way, however, Lean requires a hint that the intended monad is {anchorName mapMId}`Id`:
+```anchor mapMId
+#eval mapM (m := Id) (· + 1) [1, 2, 3, 4, 5]
+```
+```anchorInfo mapMId
+[2, 3, 4, 5, 6]
+```
+Omitting the hint results in an error:
+```anchor mapMIdNoHint
+#eval mapM (· + 1) [1, 2, 3, 4, 5]
+```
+```anchorError mapMIdNoHint
+failed to synthesize
+  HAdd Nat Nat (?m.22324 ?m.22326)
+
+Additional diagnostic information may be available using the `set_option diagnostics true` command.
+```
+In this error, the application of one metavariable to another indicates that Lean doesn't run the type-level computation backwards.
+The return type of the function is expected to be the monad applied to some other type.
+Similarly, using `mapM` with a function whose type doesn't provide any specific hints about which monad is to be used results in an “instance problem is stuck” message:
+```anchor mapMIdId
+#eval mapM (fun (x : Nat) => x) [1, 2, 3, 4, 5]
+```
+```anchorError mapMIdId
+typeclass instance problem is stuck, it is often due to metavariables
+  Monad ?m.22785
+```
+:::
+
+# The Monad Contract
+Just as every pair of instances of {anchorName MonadContract}`BEq` and {anchorName MonadContract}`Hashable` should ensure that any two equal values have the same hash, there is a contract that each instance of {anchorName MonadContract}`Monad` should obey.
+First, {anchorName MonadContract}`pure` should be a left identity of {anchorName MonadContract}`bind`.
+That is, `bind (pure v) f` should be the same as {anchorTerm MonadContract}`f v`.
+Secondly, {anchorName MonadContract}`pure` should be a right identity of {anchorName MonadContract}`bind`, so {anchorTerm MonadContract}`bind v pure` is the same as {anchorName MonadContract2}`v`.
+Finally, {anchorName MonadContract}`bind` should be associative, so {anchorTerm MonadContract}`bind (bind v f) g` is the same as {anchorTerm MonadContract}`bind v (fun x => bind (f x) g)`.
+
+This contract specifies the expected properties of programs with effects more generally.
+Because {anchorName MonadContract}`pure` has no effects, sequencing its effects with {anchorName MonadContract}`bind` shouldn't change the result.
+The associative property of {anchorName MonadContract}`bind` basically says that the sequencing bookkeeping itself doesn't matter, so long as the order in which things are happening is preserved.
+
+# Exercises
+
+## Mapping on a Tree
+
+:::paragraph
+Define a function {anchorName ex1}`BinTree.mapM`.
+By analogy to {anchorName mapM}`mapM` for lists, this function should apply a monadic function to each data entry in a tree, as a preorder traversal.
+The type signature should be:
+```anchorTerm ex1
+def BinTree.mapM [Monad m] (f : α → m β) : BinTree α → m (BinTree β)
+```
+:::
+
+## The Option Monad Contract
+
+:::paragraph
+First, write a convincing argument that the {anchorName badOptionMonad}`Monad` instance for {anchorName badOptionMonad}`Option` satisfies the monad contract.
+Then, consider the following instance:
+```anchor badOptionMonad
+instance : Monad Option where
+  pure x := some x
+  bind opt next := none
+```
+Both methods have the correct type.
+Why does this instance violate the monad contract?
+:::
