book/FPLean/TypeClasses/Conveniences.lean
@@ -1,0 +1,102 @@
+import VersoManual
+import FPLean.Examples
+
+open Verso.Genre Manual ExternalLean
+
+open FPLean
+
+set_option verso.exampleProject "../examples"
+set_option verso.exampleModule "Examples.Classes"
+
+set_option pp.rawOnError true
+
+
+#doc (Manual) "Additional Conveniences" =>
+
+
+# Constructor Syntax for Instances
+
+Behind the scenes, type classes are structure types and instances are values of these types.
+The only differences are that Lean stores additional information about type classes, such as which parameters are output parameters, and that instances are registered for searching.
+While values that have structure types are typically defined using either `⟨...⟩` syntax or with braces and fields, and instances are typically defined using {kw}`where`, both syntaxes work for both kinds of definition.
+
+:::paragraph
+For example, a forestry application might represent trees as follows:
+
+```anchor trees
+structure Tree : Type where
+  latinName : String
+  commonNames : List String
+
+def oak : Tree :=
+  ⟨"Quercus robur", ["common oak", "European oak"]⟩
+
+def birch : Tree :=
+  { latinName := "Betula pendula",
+    commonNames := ["silver birch", "warty birch"]
+  }
+
+def sloe : Tree where
+  latinName := "Prunus spinosa"
+  commonNames := ["sloe", "blackthorn"]
+```
+All three syntaxes are equivalent.
+:::
+
+:::paragraph
+Similarly, type class instances can be defined using all three syntaxes:
+
+```anchor Display
+class Display (α : Type) where
+  displayName : α → String
+
+instance : Display Tree :=
+  ⟨Tree.latinName⟩
+
+instance : Display Tree :=
+  { displayName := Tree.latinName }
+
+instance : Display Tree where
+  displayName t := t.latinName
+```
+
+The {kw}`where` syntax is typically used for instances, while structures use either the curly-brace syntax or the {kw}`where` syntax.
+The `⟨...⟩` syntax can be useful when emphasizing that a structure type is very much like a tuple in which the fields happen to be named, but the names are not important at the moment.
+However, there are situations where it can make sense to use other alternatives.
+In particular, a library might provide a function that constructs an instance value.
+Placing a call to this function after `:=` in an instance declaration is the easiest way to use such a function.
+:::
+
+# Examples
+
+When experimenting with Lean code, definitions can be more convenient to use than {kw}`#eval` or {kw}`#check` commands.
+First off, definitions don't produce any output, which can help keep the reader's focus on the most interesting output.
+Secondly, it's easiest to write most Lean programs by starting with a type signature, allowing Lean to provide more assistance and better error messages while writing the program itself.
+On the other hand, {kw}`#eval` and {kw}`#check` are easiest to use in contexts where Lean is able to determine the type from the provided expression.
+Thirdly, {kw}`#eval` cannot be used with expressions whose types don't have {moduleName}`ToString` or {moduleName}`Repr` instances, such as functions.
+Finally, multi-step {kw}`do` blocks, {kw}`let`-expressions, and other syntactic forms that take multiple lines are particularly difficult to write with a type annotation in {kw}`#eval` or {kw}`#check`, simply because the required parenthesization can be difficult to predict.
+
+:::paragraph
+To work around these issues, Lean supports the explicit indication of examples in a source file.
+An example is like a definition without a name.
+For instance, a non-empty list of birds commonly found in Copenhagen's green spaces can be written:
+
+```anchor birdExample
+example : NonEmptyList String :=
+  { head := "Sparrow",
+    tail := ["Duck", "Swan", "Magpie", "Eurasian coot", "Crow"]
+  }
+```
+:::
+
+:::paragraph
+Examples may define functions by accepting arguments:
+
+```anchor commAdd
+example (n : Nat) (k : Nat) : Bool :=
+  n + k == k + n
+```
+While this creates a function behind the scenes, this function has no name and cannot be called.
+Nonetheless, this is useful for demonstrating how a library can be used with arbitrary or unknown values of some given type.
+In source files, {kw}`example` declarations are best paired with comments that explain how the example illustrates the concepts of the library.
+:::
