book/FPLean/TypeClasses/Polymorphism.lean
@@ -1,0 +1,168 @@
+import VersoManual
+import FPLean.Examples
+
+open Verso.Genre Manual ExternalLean
+
+open FPLean
+
+set_option verso.exampleProject "../examples"
+set_option verso.exampleModule "Examples.Classes"
+
+set_option pp.rawOnError true
+
+#doc (Manual) "Type Classes and Polymorphism" =>
+
+It can be useful to write functions that work for _any_ overloading of a given function.
+For example, {anchorTerm printlnType}`IO.println` works for any type that has an instance of {anchorTerm printlnType}`ToString`.
+This is indicated using square brackets around the required instance: the type of {anchorTerm printlnType}`IO.println` is {anchorTerm printlnType}`{α : Type} → [ToString α] → α → IO Unit`.
+This type says that {anchorTerm printlnType}`IO.println` accepts an argument of type {anchorTerm printlnType}`α`, which Lean should determine automatically, and that there must be a {anchorTerm printlnType}`ToString` instance available for {anchorTerm printlnType}`α`.
+It returns an {anchorTerm printlnType}`IO` action.
+
+
+# Checking Polymorphic Functions' Types
+
+Checking the type of a function that takes implicit arguments or uses type classes requires the use of some additional syntax.
+Simply writing
+```anchor printlnMetas
+#check (IO.println)
+```
+yields a type with metavariables:
+```anchorInfo printlnMetas
+IO.println : ?m.2620 → IO Unit
+```
+This is because Lean does its best to discover implicit arguments, and the presence of metavariables indicates that it did not yet discover enough type information to do so.
+To understand the signature of a function, this feature can be suppressed with an at-sign (`@`) before the function's name:
+```anchor printlnNoMetas
+#check @IO.println
+```
+```anchorInfo printlnNoMetas
+@IO.println : {α : Type u_1} → [inst : ToString α] → α → IO Unit
+```
+In this output, the instance itself has been given the name `inst`.
+Additionally, there is a `u_1` after `Type`, which uses a feature of Lean that has not yet been introduced.
+For now, ignore these parameters to {moduleTerm}`Type`.
+
+# Defining Polymorphic Functions with Instance Implicits
+
+A function that sums all entries in a list needs two instances: {moduleName}`Add` allows the entries to be added, and an {moduleName}`OfNat` instance for `0` provides a sensible value to return for the empty list:
+
+```anchor ListSum
+def List.sumOfContents [Add α] [OfNat α 0] : List α → α
+  | [] => 0
+  | x :: xs => x + xs.sumOfContents
+```
+This function can be also defined with a {anchorTerm ListSumZ}`Zero α` requirement instead of {anchorTerm ListSum}`OfNat α 0`.
+Both are equivalent, but {anchorTerm ListSumZ}`Zero α` can be easier to read:
+
+```anchor ListSumZ
+def List.sumOfContents [Add α] [Zero α] : List α → α
+  | [] => 0
+  | x :: xs => x + xs.sumOfContents
+```
+
+This function can be used for a list of {anchorTerm fourNats}`Nat`s:
+
+```anchor fourNats
+def fourNats : List Nat := [1, 2, 3, 4]
+```
+```anchor fourNatsSum
+#eval fourNats.sumOfContents
+```
+```anchorInfo fourNatsSum
+10
+```
+but not for a list of {anchorTerm fourPos}`Pos` numbers:
+
+```anchor fourPos
+def fourPos : List Pos := [1, 2, 3, 4]
+```
+```anchor fourPosSum
+#eval fourPos.sumOfContents
+```
+```anchorError fourPosSum
+failed to synthesize
+  Zero Pos
+
+Additional diagnostic information may be available using the `set_option diagnostics true` command.
+```
+The Lean standard library includes this function, where it is called {moduleName}`List.sum`.
+
+Specifications of required instances in square brackets are called _instance implicits_.
+Behind the scenes, every type class defines a structure that has a field for each overloaded operation.
+Instances are values of that structure type, with each field containing an implementation.
+At a call site, Lean is responsible for finding an instance value to pass for each instance implicit argument.
+The most important difference between ordinary implicit arguments and instance implicits is the strategy that Lean uses to find an argument value.
+In the case of ordinary implicit arguments, Lean uses a technique called _unification_ to find a single unique argument value that would allow the program to pass the type checker.
+This process relies only on the specific types involved in the function's definition and the call site.
+For instance implicits, Lean instead consults a built-in table of instance values.
+
+Just as the {anchorTerm OfNatPos}`OfNat` instance for {anchorName OfNatPos}`Pos` took a natural number {anchorName OfNatPos}`n` as an automatic implicit argument, instances may also take instance implicit arguments themselves.
+The [section on polymorphism](../getting-to-know/polymorphism.md) presented a polymorphic point type:
+
+```anchor PPoint
+structure PPoint (α : Type) where
+  x : α
+  y : α
+deriving Repr
+```
+Addition of points should add the underlying {anchorName PPoint}`x` and {anchorName PPoint}`y` fields.
+Thus, an {anchorName AddPPoint}`Add` instance for {anchorName AddPPoint}`PPoint` requires an {anchorName AddPPoint}`Add` instance for whatever type these fields have.
+In other words, the {anchorName AddPPoint}`Add` instance for {anchorName AddPPoint}`PPoint` requires a further {anchorName AddPPoint}`Add` instance for {anchorName AddPPoint}`α`:
+
+```anchor AddPPoint
+instance [Add α] : Add (PPoint α) where
+  add p1 p2 := { x := p1.x + p2.x, y := p1.y + p2.y }
+```
+When Lean encounters an addition of two points, it searches for and finds this instance.
+It then performs a further search for the {anchorTerm AddPPoint}`Add α` instance.
+
+The instance values that are constructed in this way are values of the type class's structure type.
+A successful recursive instance search results in a structure value that has a reference to another structure value.
+An instance of {moduleTerm}`Add (PPoint Nat)` contains a reference to the instance of {moduleTerm}`Add Nat` that was found.
+
+This recursive search process means that type classes offer significantly more power than plain overloaded functions.
+A library of polymorphic instances is a set of code building blocks that the compiler will assemble on its own, given nothing but the desired type.
+Polymorphic functions that take instance arguments are latent requests to the type class mechanism to assemble helper functions behind the scenes.
+The API's clients are freed from the burden of plumbing together all of the necessary parts by hand.
+
+
+# Methods and Implicit Arguments
+
+
+The type of {anchorTerm ofNatType}`OfNat.ofNat` may be surprising.
+It is {anchorTerm ofNatType}`: {α : Type} → (n : Nat) → [OfNat α n] → α`, in which the {anchorTerm ofNatType}`Nat` argument {anchorTerm ofNatType}`n` occurs as an explicit function parameter.
+In the declaration of the method, however, {anchorName OfNat}`ofNat` simply has type {anchorName ofNatType}`α`.
+This seeming discrepancy is because declaring a type class really results in the following:
+
+ * A structure type to contain the implementation of each overloaded operation
+ * A namespace with the same name as the class
+ * For each method, a function in the class's namespace that retrieves its implementation from an instance
+
+This is analogous to the way that declaring a new structure also declares accessor functions.
+The primary difference is that a structure's accessors take the structure value as an explicit parameter, while the type class methods take the instance value as an instance implicit to be found automatically by Lean.
+
+In order for Lean to find an instance, its parameters must be available.
+This means that each parameter to the type class must be a parameter to the method that occurs before the instance.
+It is most convenient when these parameters are implicit, because Lean does the work of discovering their values.
+For example, {anchorTerm addType}`Add.add` has the type {anchorTerm addType}`{α : Type} → [Add α] → α → α → α`.
+In this case, the type parameter {anchorTerm addType}`α` can be implicit because the arguments to {anchorTerm addType}`Add.add` provide information about which type the user intended.
+This type can then be used to search for the {anchorTerm addType}`Add` instance.
+
+In the case of {anchorName ofNatType}`OfNat.ofNat`, however, the particular {moduleName}`Nat` literal to be decoded does not appear as part of any other parameter's type.
+This means that Lean would have no information to use when attempting to figure out the implicit parameter {anchorName ofNatType}`n`.
+The result would be a very inconvenient API.
+Thus, in these cases, Lean uses an explicit parameter for the class's method.
+
+
+
+# Exercises
+
+## Even Number Literals
+
+Write an instance of {anchorName ofNatType}`OfNat` for the even number datatype from the [previous section's exercises](pos.md#even-numbers) that uses recursive instance search.
+
+## Recursive Instance Search Depth
+
+There is a limit to how many times the Lean compiler will attempt a recursive instance search.
+This places a limit on the size of even number literals defined in the previous exercise.
+Experimentally determine what the limit is.
