book/FPLean/TypeClasses/Pos.lean
@@ -1,0 +1,391 @@
+import VersoManual
+import FPLean.Examples
+
+open Verso.Genre Manual ExternalLean
+
+open FPLean
+
+set_option verso.exampleProject "../examples"
+set_option verso.exampleModule "Examples.Classes"
+
+set_option pp.rawOnError true
+
+#doc (Manual) "Positive Numbers" =>
+
+In some applications, only positive numbers make sense.
+For example, compilers and interpreters typically use one-indexed line and column numbers for source positions, and a datatype that represents only non-empty lists will never report a length of zero.
+Rather than relying on natural numbers, and littering the code with assertions that the number is not zero, it can be useful to design a datatype that represents only positive numbers.
+
+One way to represent positive numbers is very similar to {moduleTerm}`Nat`, except with {anchorTerm Pos}`one` as the base case instead of {anchorTerm Nat.zero}`zero`:
+
+```anchor Pos
+inductive Pos : Type where
+  | one : Pos
+  | succ : Pos → Pos
+```
+This datatype represents exactly the intended set of values, but it is not very convenient to use.
+For example, numeric literals are rejected:
+```anchor sevenOops
+def seven : Pos := 7
+```
+```anchorError sevenOops
+failed to synthesize
+  OfNat Pos 7
+numerals are polymorphic in Lean, but the numeral `7` cannot be used in a context where the expected type is
+  Pos
+due to the absence of the instance above
+
+Additional diagnostic information may be available using the `set_option diagnostics true` command.
+```
+Instead, the constructors must be used directly:
+```anchor seven
+def seven : Pos :=
+  Pos.succ (Pos.succ (Pos.succ (Pos.succ (Pos.succ (Pos.succ Pos.one)))))
+```
+
+Similarly, addition and multiplication are not easy to use:
+```anchor fourteenOops
+def fourteen : Pos := seven + seven
+```
+```anchorError fourteenOops
+failed to synthesize
+  HAdd Pos Pos ?m.543
+
+Additional diagnostic information may be available using the `set_option diagnostics true` command.
+```
+```anchor fortyNineOops
+def fortyNine : Pos := seven * seven
+```
+```anchorError fortyNineOops
+failed to synthesize
+  HMul Pos Pos ?m.576
+
+Additional diagnostic information may be available using the `set_option diagnostics true` command.
+```
+
+Each of these error messages begins with `failed to synthesize instance`.
+This indicates that the error is due to an overloaded operation that has not been implemented, and it describes the type class that must be implemented.
+
+# Classes and Instances
+
+A type class consists of a name, some parameters, and a collection of {tech}_methods_.
+The parameters describe the types for which overloadable operations are being defined, and the methods are the names and type signatures of the overloadable operations.
+Once again, there is a terminology clash with object-oriented languages.
+In object-oriented programming, a method is essentially a function that is connected to a particular object in memory, with special access to the object's private state.
+Objects are interacted with via their methods.
+In Lean, the term "method" refers to an operation that has been declared to be overloadable, with no special connection to objects or values or private fields.
+
+One way to overload addition is to define a type class named {anchorName Plus}`Plus`, with an addition method named `plus`.
+Once an instance of {anchorTerm Plus}`Plus` for {moduleTerm}`Nat` has been defined, it becomes possible to add two {moduleTerm}`Nat`s using {anchorName plusNatFiveThree}`Plus.plus`:
+```anchor plusNatFiveThree
+#eval Plus.plus 5 3
+```
+```anchorInfo plusNatFiveThree
+8
+```
+Adding more instances allows {anchorName plusNatFiveThree}`Plus.plus` to take more types of arguments.
+
+In the following type class declaration, {anchorName Plus}`Plus` is the name of the class, {anchorTerm Plus}`α : Type` is the only argument, and {anchorTerm Plus}`plus : α → α → α` is the only method:
+
+```anchor Plus
+class Plus (α : Type) where
+  plus : α → α → α
+```
+This declaration says that there is a type class {anchorName Plus}`Plus` that overloads operations with respect to a type `α`.
+In particular, there is one overloaded operation called `plus` that takes two `α`s and returns an `α`.
+
+Type classes are first class, just as types are first class.
+In particular, a type class is another kind of type.
+The type of {anchorTerm PlusType}`Plus` is {anchorTerm PlusType}`Type → Type`, because it takes a type as an argument (`α`) and results in a new type that describes the overloading of {anchorName Plus}`Plus`'s operation for `α`.
+
+
+To overload `plus` for a particular type, write an instance:
+
+```anchor PlusNat
+instance : Plus Nat where
+  plus := Nat.add
+```
+The colon after `instance` indicates that `Plus Nat` is indeed a type.
+Each method of class {anchorName Plus}`Plus` should be assigned a value using `:=`.
+In this case, there is only one method: `plus`.
+
+By default, type class methods are defined in a namespace with the same name as the type class.
+It can be convenient to `open` the namespace so that users don't need to type the name of the class first.
+Parentheses in an `open` command indicate that only the indicated names from the namespace are to be made accessible:
+
+```anchor openPlus
+open Plus (plus)
+```
+```anchor plusNatFiveThreeAgain
+#eval plus 5 3
+```
+```anchorInfo plusNatFiveThreeAgain
+8
+```
+
+Defining an addition function for `Pos` and an instance of `Plus Pos` allows `plus` to be used to add both `Pos` and {moduleTerm}`Nat` values:
+
+```anchor PlusPos
+def Pos.plus : Pos → Pos → Pos
+  | Pos.one, k => Pos.succ k
+  | Pos.succ n, k => Pos.succ (n.plus k)
+
+instance : Plus Pos where
+  plus := Pos.plus
+
+def fourteen : Pos := plus seven seven
+```
+
+Because there is not yet an instance of {moduleTerm}`Plus Float`, attempting to add two floating-point numbers with {anchorName plusFloatFail}`plus` fails with a familiar message:
+```anchor plusFloatFail
+#eval plus 5.2 917.25861
+```
+```anchorError plusFloatFail
+failed to synthesize
+  Plus Float
+
+Additional diagnostic information may be available using the `set_option diagnostics true` command.
+```
+These errors mean that Lean was unable to find an instance for a given type class.
+
+# Overloaded Addition
+
+Lean's built-in addition operator is syntactic sugar for a type class called `HAdd`, which flexibly allows the arguments to addition to have different types.
+`HAdd` is short for _heterogeneous addition_.
+For example, an `HAdd` instance can be written to allow a {moduleName}`Nat` to be added to a `Float`, resulting in a new `Float`.
+When a programmer writes {anchorTerm plusDesugar}`x + y`, it is interpreted as meaning {anchorTerm plusDesugar}`HAdd.hAdd x y`.
+
+While an understanding of the full generality of `HAdd` relies on features that are discussed in [another section in this chapter](out-params.md), there is a simpler type class called `Add` that does not allow the types of the arguments to be mixed.
+The Lean libraries are set up so that an instance of `Add` will be found when searching for an instance of `HAdd` in which both arguments have the same type.
+
+Defining an instance of {anchorTerm AddPos}`Add Pos` allows {anchorTerm AddPos}`Pos` values to use ordinary addition syntax:
+
+```anchor AddPos
+instance : Add Pos where
+  add := Pos.plus
+```
+```anchor betterFourteen
+def fourteen : Pos := seven + seven
+```
+
+# Conversion to Strings
+
+Another useful built-in class is called {anchorName UglyToStringPos}`ToString`.
+Instances of {anchorName UglyToStringPos}`ToString` provide a standard way of converting values from a given type into strings.
+For example, a {anchorName UglyToStringPos}`ToString` instance is used when a value occurs in an interpolated string, and it determines how the `IO.println` function used at the [beginning of the description of `IO`](../hello-world/running-a-program.html#running-a-program) will display a value.
+
+For example, one way to convert a `Pos` into a `String` is to reveal its inner structure.
+The function `posToString` takes a `Bool` that determines whether to parenthesize uses of `Pos.succ`, which should be `true` in the initial call to the function and `false` in all recursive calls.
+
+```anchor posToStringStructure
+def posToString (atTop : Bool) (p : Pos) : String :=
+  let paren s := if atTop then s else "(" ++ s ++ ")"
+  match p with
+  | Pos.one => "Pos.one"
+  | Pos.succ n => paren s!"Pos.succ {posToString false n}"
+```
+Using this function for a {anchorName UglyToStringPos}`ToString` instance:
+
+```anchor UglyToStringPos
+instance : ToString Pos where
+  toString := posToString true
+```
+results in informative, yet overwhelming, output:
+```anchor sevenLong
+#eval s!"There are {seven}"
+```
+```anchorInfo sevenLong
+"There are Pos.succ (Pos.succ (Pos.succ (Pos.succ (Pos.succ (Pos.succ Pos.one)))))"
+```
+
+On the other hand, every positive number has a corresponding {moduleTerm}`Nat`.
+Converting it to a {moduleTerm}`Nat` and then using the {moduleTerm}`ToString Nat` instance (that is, the overloading of {anchorName UglyToStringPos}`ToString` for {moduleTerm}`Nat`) is a quick way to generate much shorter output:
+
+```anchor posToNat
+def Pos.toNat : Pos → Nat
+  | Pos.one => 1
+  | Pos.succ n => n.toNat + 1
+```
+```anchor PosToStringNat
+instance : ToString Pos where
+  toString x := toString (x.toNat)
+```
+```anchor sevenShort
+#eval s!"There are {seven}"
+```
+```anchorInfo sevenShort
+"There are 7"
+```
+When more than one instance is defined, the most recent takes precedence.
+Additionally, if a type has a {anchorName UglyToStringPos}`ToString` instance, then it can be used to display the result of {kw}`#eval` even if the type in question was not defined with `deriving Repr`, so {anchorTerm sevenEvalStr}`#eval seven` outputs {anchorInfo sevenEvalStr}`7`.
+
+# Overloaded Multiplication
+
+For multiplication, there is a type class called `HMul` that allows mixed argument types, just like `HAdd`.
+Just as {anchorTerm plusDesugar}`x + y` is interpreted as {anchorTerm plusDesugar}[`HAdd.hAdd x y`], {anchorTerm timesDesugar}`x * y` is interpreted as {anchorTerm timesDesugar}`HMul.hMul x y`.
+For the common case of multiplication of two arguments with the same type, a {moduleTerm}`Mul` instance suffices.
+
+An instance of {moduleTerm}`Mul` allows ordinary multiplication syntax to be used with {moduleTerm}`Pos`:
+
+```anchor PosMul
+def Pos.mul : Pos → Pos → Pos
+  | Pos.one, k => k
+  | Pos.succ n, k => n.mul k + k
+
+instance : Mul Pos where
+  mul := Pos.mul
+```
+With this instance, multiplication works as expected:
+```anchor muls
+#eval [seven * Pos.one,
+       seven * seven,
+       Pos.succ Pos.one * seven]
+```
+```anchorInfo muls
+[7, 49, 14]
+```
+
+# Literal Numbers
+
+It is quite inconvenient to write out a sequence of constructors for positive numbers.
+One way to work around the problem would be to provide a function to convert a {moduleTerm}`Nat` into a `Pos`.
+However, this approach has downsides.
+First off, because {moduleTerm}`Pos` cannot represent `0`, the resulting function would either convert a {moduleTerm}`Nat` to a bigger number, or it would return {moduleTerm}`Option Pos`.
+Neither is particularly convenient for users.
+Secondly, the need to call the function explicitly would make programs that use positive numbers much less convenient to write than programs that use {moduleTerm}`Nat`.
+Having a trade-off between precise types and convenient APIs means that the precise types become less useful.
+
+There are two type classes that are used to overload numeric literals: {moduleName}`Zero` and {moduleName}`OfNat`.
+Because many types have values that are naturally written with `0`, the {moduleName}`Zero` class allow these specific values to be overridden.
+It is defined as follows:
+
+```anchor Zero
+class Zero (α : Type) where
+  zero : α
+```
+Because `0` is not a positive number, there should be no instance of {moduleTerm}`Zero Pos`.
+
+In Lean, natural number literals are interpreted using a type class called {moduleName}`OfNat`:
+
+```anchor OfNat
+class OfNat (α : Type) (_ : Nat) where
+  ofNat : α
+```
+This type class takes two arguments: {anchorTerm OfNat}`α` is the type for which a natural number is overloaded, and the unnamed {moduleTerm}`Nat` argument is the actual literal number that was encountered in the program.
+The method {anchorName OfNat}`ofNat` is then used as the value of the numeric literal.
+Because the class contains the {moduleTerm}`Nat` argument, it becomes possible to define only instances for those values where the number makes sense.
+
+{anchorTerm OfNat}`OfNat` demonstrates that the arguments to type classes do not need to be types.
+Because types in Lean are first-class participants in the language that can be passed as arguments to functions and given definitions with {kw}`def` and {kw}`abbrev`, there is no barrier that prevents non-type arguments in positions where a less-flexible language could not permit them.
+This flexibility allows overloaded operations to be provided for particular values as well as particular types.
+Additionally, it allows the Lean standard library to arrange for there to be a {moduleTerm}`Zero α` instance whenever there's an {moduleTerm}`OfNat α 0` instance, and vice versa.
+
+A sum type that represents natural numbers less than four can be defined as follows:
+
+```anchor LT4
+inductive LT4 where
+  | zero
+  | one
+  | two
+  | three
+deriving Repr
+```
+While it would not make sense to allow _any_ literal number to be used for this type, numbers less than four clearly make sense:
+
+```anchor LT4ofNat
+instance : OfNat LT4 0 where
+  ofNat := LT4.zero
+
+instance : OfNat LT4 1 where
+  ofNat := LT4.one
+
+instance : OfNat LT4 2 where
+  ofNat := LT4.two
+
+instance : OfNat LT4 3 where
+  ofNat := LT4.three
+```
+With these instances, the following examples work:
+```anchor LT4three
+#eval (3 : LT4)
+```
+```anchorInfo LT4three
+LT4.three
+```
+```anchor LT4zero
+#eval (0 : LT4)
+```
+```anchorInfo LT4zero
+LT4.zero
+```
+On the other hand, out-of-bounds literals are still not allowed:
+```anchor LT4four
+#eval (4 : LT4)
+```
+```anchorError LT4four
+failed to synthesize
+  OfNat LT4 4
+numerals are polymorphic in Lean, but the numeral `4` cannot be used in a context where the expected type is
+  LT4
+due to the absence of the instance above
+
+Additional diagnostic information may be available using the `set_option diagnostics true` command.
+```
+
+For {moduleTerm}`Pos`, the {anchorTerm OfNat}`OfNat` instance should work for _any_ {moduleTerm}`Nat` other than {moduleTerm}`Nat.zero`.
+Another way to phrase this is to say that for all natural numbers {anchorTerm posrec}`n`, the instance should work for {anchorTerm posrec}`n + 1`.
+Just as names like {anchorTerm posrec}`α` automatically become implicit arguments to functions that Lean fills out on its own, instances can take automatic implicit arguments.
+In this instance, the argument {anchorTerm OfNatPos}`n` stands for any {moduleTerm}`Nat`, and the instance is defined for a {moduleTerm}`Nat` that's one greater:
+
+```anchor OfNatPos
+instance : OfNat Pos (n + 1) where
+  ofNat :=
+    let rec natPlusOne : Nat → Pos
+      | 0 => Pos.one
+      | k + 1 => Pos.succ (natPlusOne k)
+    natPlusOne n
+```
+Because {anchorTerm OfNatPos}`n` stands for a {moduleTerm}`Nat` that's one less than what the user wrote, the helper function {anchorName OfNatPos}`natPlusOne` returns a {anchorName OfNatPos}`Pos` that's one greater than its argument.
+This makes it possible to use natural number literals for positive numbers, but not for zero:
+
+```anchor eight
+def eight : Pos := 8
+```
+```anchor zeroBad
+def zero : Pos := 0
+```
+```anchorError zeroBad
+failed to synthesize
+  OfNat Pos 0
+numerals are polymorphic in Lean, but the numeral `0` cannot be used in a context where the expected type is
+  Pos
+due to the absence of the instance above
+
+Additional diagnostic information may be available using the `set_option diagnostics true` command.
+```
+
+# Exercises
+
+## Another Representation
+
+An alternative way to represent a positive number is as the successor of some {moduleTerm}`Nat`.
+Replace the definition of {moduleName}`Pos` with a structure whose constructor is named {anchorName AltPos}`succ` that contains a {moduleTerm}`Nat`:
+
+```anchor AltPos
+structure Pos where
+  succ ::
+  pred : Nat
+```
+Define instances of {moduleName}`Add`, {moduleName}`Mul`, {anchorName UglyToStringPos}`ToString`, and {moduleName}`OfNat` that allow this version of {anchorName AltPos}`Pos` to be used conveniently.
+
+## Even Numbers
+
+Define a datatype that represents only even numbers. Define instances of {moduleName}`Add`, {moduleName}`Mul`, and {anchorName UglyToStringPos}`ToString` that allow it to be used conveniently.
+{moduleName}`OfNat` requires a feature that is introduced in [the next section](polymorphism.md).
+
+## HTTP Requests
+
+An HTTP request begins with an identification of a HTTP method, such as `GET` or `POST`, along with a URI and an HTTP version.
+Define an inductive type that represents an interesting subset of the HTTP methods, and a structure that represents HTTP responses.
+Responses should have a {anchorName UglyToStringPos}`ToString` instance that makes it possible to debug them.
+Use a type class to associate different {moduleName}`IO` actions with each HTTP method, and write a test harness as an {moduleName}`IO` action that calls each method and prints the result.
